fix compilation for SSReflect 1.11 + warnings

Core/pperm.v
@@ -1,4 +1,4 @@
-Require Import ssreflect ssrfun. 
+Require Import ssreflect ssrfun.
 From mathcomp.ssreflect Require Import ssrbool ssrnat seq eqtype path.
 From HTT Require Import pred.
 Set Implicit Arguments.
@@ -12,284 +12,187 @@ Import Prenex Implicits.
 Section Permutations.
 Variable A : Type.
 
-Lemma in_split (x : A) (s : seq A) :
-        x \In s -> exists s1, exists s2, s = s1 ++ x :: s2.
+Inductive perm : seq A -> seq A -> Prop :=
+| permutation_nil : perm [::] [::]
+| permutation_skip x s1 s2 of perm s1 s2 : perm (x :: s1) (x :: s2)
+| permutation_swap x y s1 s2 of perm s1 s2 : perm [:: x, y & s1] [:: y, x & s2]
+| permutation_trans t s1 s2 of perm s1 t & perm t s2 : perm s1 s2.
+
+Lemma pperm_refl (s : seq A) : perm s s.
+Proof. by elim: s=>*; [apply: permutation_nil | apply: permutation_skip]. Qed.
+
+Hint Resolve pperm_refl : core.
+
+Lemma pperm_nil (s : seq A) : perm [::] s <-> s = [::].
 Proof.
-elim:s=>[|y s IH] //=; rewrite InE.
-case=>[<-|]; first by exists [::]; exists s.
-by case/IH=>s1 [s2] ->; exists (y :: s1); exists s2.
+split; last by move=>->; apply: permutation_nil.
+move E: {1}[::]=>l H; move: H {E}(esym E).
+by elim=>//??? _ IH1 _ IH2 /IH1/IH2.
 Qed.
 
-Inductive perm (s1 s2 : seq A) : Prop :=
-| permutation_nil of s1 = [::] & s2 = [::]
-| permutation_skip x t1 t2 of s1 = x :: t1 & s2 = x :: t2 & perm t1 t2
-| permutation_swap x y t of s1 = x :: y :: t & s2 = y :: x :: t
-| permutation_trans t of perm s1 t & perm t s2.
-
-Lemma perm_nil (s : seq A) : perm [::] s <-> s = [::].
+Lemma pperm_sym s1 s2 : perm s1 s2 <-> perm s2 s1.
 Proof.
-split=>[H|]; last by move=>->; apply: permutation_nil.
-move: {1 2}[::] s H (erefl (Nil A)).
-apply: perm_ind=>[|s1 s2 x t1 t2 ->|s1 s2 x y t ->|s1 s2 t _ IH1 _ IH2] //.
-by move/IH1; move/IH2.
+suff {s1 s2} L : forall s1 s2, perm s1 s2 -> perm s2 s1 by split; apply: L.
+apply: perm_ind=>[|||??? _ H1 _ H2] *;
+by [apply: permutation_nil | apply: permutation_skip |
+    apply: permutation_swap | apply: permutation_trans H2 H1].
 Qed.
 
-Lemma perm_refl (s : seq A) : perm s s.
-Proof.
-elim:s=>[|e s IH]; first by apply: permutation_nil.
-by apply: (permutation_skip (x:=e)) IH.
-Qed.
-
-Hint Resolve perm_refl.
-
-Lemma perm_sym s1 s2 : perm s1 s2 <-> perm s2 s1.
-Proof.
-suff L: forall s1 s2, perm s1 s2 -> perm s2 s1 by split; apply: L.
-apply: perm_ind=>s1' s2'.
-- by move=>->->; apply: permutation_nil.
-- by move=>x t1 t2 -> -> H1; apply: permutation_skip.
-- by move=>x y t -> ->; apply: permutation_swap.
-by move=>t _ H1 _ H2; apply: permutation_trans H2 H1.
-Qed.
-
-Lemma perm_trans s2 s1 s3 : perm s1 s2 -> perm s2 s3 -> perm s1 s3.
+Lemma pperm_trans s2 s1 s3 : perm s1 s2 -> perm s2 s3 -> perm s1 s3.
 Proof. by apply: permutation_trans. Qed.
 
-Lemma perm_in s1 s2 x : perm s1 s2 -> x \In s1 -> x \In s2.
-Proof.
-move: s1 s2; apply: perm_ind=>s1 s2.
-- by move=>->->.
-- move=>y t1 t2 -> -> H; rewrite !InE; tauto.
-- by move=>y z t -> ->; rewrite !InE; tauto.
-by move=>t _ IH1 _ IH2; move/IH1; move/IH2.
-Qed.
+Lemma pperm_in s1 s2 x : perm s1 s2 -> x \In s1 -> x \In s2.
+Proof. elim=>//??? =>[|?|_ I1 _ I2 /I1/I2]; rewrite ?InE; tauto. Qed.
 
-Lemma perm_cat2lL s s1 s2 : perm s1 s2 -> perm (s ++ s1) (s ++ s2).
-Proof. by elim:s=>[|e s IH] //=; move/IH; apply: permutation_skip. Qed.
-
-Lemma perm_cat2rL s s1 s2 : perm s1 s2 -> perm (s1 ++ s) (s2 ++ s).
+Lemma pperm_catC s1 s2 : perm (s1 ++ s2) (s2 ++ s1).
 Proof.
-move=>H; move: s1 s2 H s; apply: perm_ind=>s1 s2.
-- by move=>->->.
-- by move=>x t1 t2 -> -> H IH s /=; apply: permutation_skip.
-- by move=>x y t -> -> s /=; apply: permutation_swap.
-by move=>t H1 IH1 H2 IH2 s; apply: permutation_trans (IH2 s).
-Qed.
-
-Lemma perm_catL s1 t1 s2 t2 :
-        perm s1 s2 -> perm t1 t2 -> perm (s1 ++ t1) (s2 ++ t2).
-Proof.
-move=>H; move: s1 s2 H t1 t2; apply: perm_ind=>s1 s2.
-- by move=>->->.
-- move=>x t1 t2 -> -> H IH r1 r2.
-  by move/IH; apply: permutation_skip.
-- move=>x y t -> -> t1 t2 H.
-  by apply: (permutation_trans (t:=[:: x, y & t] ++ t2));
-     [apply: perm_cat2lL | simpl; apply: permutation_swap].
-move=>t H1 IH1 H2 IH2 t1 t2 H.
-by apply: permutation_trans (IH2 _ _ H); apply: IH1.
-Qed.
-
-Lemma perm_cat_consL s1 t1 s2 t2 x :
-        perm s1 s2 -> perm t1 t2 -> perm (s1 ++ x :: t1) (s2 ++ x :: t2).
-Proof.
-by move=>H1 H2; apply: perm_catL H1 _; apply: permutation_skip H2.
-Qed.
-
-Lemma perm_catC s1 s2 : perm (s1 ++ s2) (s2 ++ s1).
-Proof.
-elim:s1 s2=>[|x s1 IH1] s2 /=; first by rewrite cats0.
-apply: (@perm_trans (x::s2++s1)); first by apply: permutation_skip (IH1 s2).
+elim: s1 s2=>[|x s1 IH1] s2 /=; first by rewrite cats0.
+apply: (@pperm_trans (x::s2++s1)); first by apply: permutation_skip.
 elim: s2=>[|y s2 IH2] //=.
-apply: (@perm_trans (y::x::s2++s1)); first by apply: permutation_swap.
-by apply: permutation_skip IH2.
+apply: (@pperm_trans (y::x::s2++s1)); first by apply: permutation_swap.
+by apply: permutation_skip.
 Qed.
 
-Hint Resolve perm_catC.
+Hint Resolve pperm_catC : core.
 
-Lemma perm_cons_catCA s1 s2 x : perm (x :: s1 ++ s2) (s1 ++ x :: s2).
+Lemma pperm_cat2lL s s1 s2 : perm s1 s2 -> perm (s ++ s1) (s ++ s2).
+Proof. by elim: s=>[//|e s IH /IH]; apply: permutation_skip. Qed.
+
+Lemma pperm_cat2rL s s1 s2 : perm s1 s2 -> perm (s1 ++ s) (s2 ++ s).
 Proof.
-rewrite -cat_rcons -cats1 -cat_cons -cat1s.
-by apply: perm_cat2rL; apply: perm_catC.
+move=>?.
+apply: (@pperm_trans (s ++ s1)); first by apply: pperm_catC.
+apply: (@pperm_trans (s ++ s2)); last by apply: pperm_catC.
+by apply: pperm_cat2lL.
 Qed.
 
-Lemma perm_cons_catAC s1 s2 x : perm (s1 ++ x :: s2) (x :: s1 ++ s2).
-Proof. by apply/perm_sym; apply: perm_cons_catCA. Qed.
+Lemma pperm_catL s1 t1 s2 t2 :
+        perm s1 s2 -> perm t1 t2 -> perm (s1 ++ t1) (s2 ++ t2).
+Proof. by move/(pperm_cat2rL t1)=>H1/(pperm_cat2lL s2); apply: pperm_trans. Qed.
 
-Hint Resolve perm_cons_catCA perm_cons_catAC.
+Lemma pperm_cat_consL s1 t1 s2 t2 x :
+        perm s1 s2 -> perm t1 t2 -> perm (s1 ++ x :: t1) (s2 ++ x :: t2).
+Proof. by move=>*; apply: pperm_catL=>//; apply: permutation_skip. Qed.
 
-Lemma perm_cons_cat_consL s1 s2 s x :
+Lemma pperm_cons_catCA s1 s2 x : perm (x :: s1 ++ s2) (s1 ++ x :: s2).
+Proof.
+rewrite -cat1s -(cat1s _ s2) !catA.
+by apply/pperm_cat2rL/pperm_catC.
+Qed.
+
+Lemma pperm_cons_catAC s1 s2 x : perm (s1 ++ x :: s2) (x :: s1 ++ s2).
+Proof. by apply/pperm_sym/pperm_cons_catCA. Qed.
+
+Hint Resolve pperm_cons_catCA pperm_cons_catAC : core.
+
+Lemma pperm_cons_cat_consL s1 s2 s x :
         perm s (s1 ++ s2) -> perm (x :: s) (s1 ++ x :: s2).
 Proof.
-case: s1=>[|a s1] /= H; first by apply: permutation_skip.
-apply: (@perm_trans (x::a::s1++s2)); first by apply: permutation_skip.
-apply: (@perm_trans (a::x::s1++s2)); first by apply: permutation_swap.
-by apply: permutation_skip=>//; apply: perm_catCA.
+move=>?.
+apply: (@pperm_trans (x :: (s1 ++ s2))); first by apply: permutation_skip.
+by apply: pperm_cons_catCA.
 Qed.
 
-(* a somewhat generalized induction principle *)
-Lemma perm_ind2 (P : seq A -> seq A -> Prop) :
-        P [::] [::] ->
-        (forall x s1 s2, perm s1 s2 -> P s1 s2 ->
-           P (x :: s1) (x :: s2)) ->
-        (forall x y s1 s2, perm s1 s2 -> P s1 s2 ->
-           P (y :: x :: s1) (x :: y :: s2)) ->
-        (forall s2 s1 s3, perm s1 s2 -> P s1 s2 ->
-           perm s2 s3 -> P s2 s3 -> P s1 s3) ->
-        forall s1 s2, perm s1 s2 -> P s1 s2.
-Proof.
-move=>H1 H2 H3 H4; apply: perm_ind=>s1 s2; last 1 first.
-- by move=>t; apply: H4.
-- by move=>->->.
-- by move=>x t1 t2 -> ->; apply: H2.
-move=>x y t -> ->.
-have R : forall t, P t t by elim=>[|e t1 IH] //; apply:  H2.
-apply: (H4 (y :: x :: t))=>//; last by apply: H3.
-by apply: permutation_swap.
-Qed.
+Lemma pperm_size l1 l2: perm l1 l2 -> size l1 = size l2.
+Proof. by elim=>//=???? =>[|?|]->. Qed.
 
-Lemma perm_size l1 l2: perm l1 l2 -> size l1 = size l2.
-Proof.
-move: l1 l2; apply: perm_ind=>s1 s2=>[|x t1 t2|x y t|t]; first by move=>->->.
-- by move=>->->{s1 s2} _ /=->.
-- by move=>->->{s1 s2}/=.
-- by move=>_->_->.
-Qed.
-
-(* Now the hard part; the opposite implications *)
-Lemma perm_cat_consR s1 t1 s2 t2 x :
+Lemma pperm_cat_consR s1 s2 t1 t2 x :
         perm (s1 ++ x :: t1) (s2 ++ x :: t2) -> perm (s1 ++ t1) (s2 ++ t2).
 Proof.
 move: s1 t1 s2 t2 x.
 suff H:
   forall r1 r2, perm r1 r2 -> forall x s1 t1 s2 t2,
     r1 = s1 ++ x :: t1 -> r2 = s2 ++ x :: t2 -> perm (s1 ++ t1) (s2 ++ t2).
-- by move=>s1 t1 s2 t2 x; move/H; apply.
-apply: perm_ind2; last 1 first.
+- by move=>s1 t1 s2 t2 x /H; apply.
+apply: perm_ind; last 1 first.
 - move=>s2 s1 s3 H1 IH1 H2 IH2 x r1 t1 r2 t2 E1 E2.
-  case: (@in_split x s2).
-  - apply: perm_in H1 _; rewrite E1; apply: (@perm_in (x::r1++t1))=>//.
-  by rewrite InE; left.
-  move=>s4 [s5] E; apply: (@perm_trans (s4++s5)); first by apply: IH1 E1 E.
+  case: (@In_split _ x s2).
+  - by apply: pperm_in H1 _; rewrite E1 Mem_cat; right; left.
+  move=>s4 [s5] E; apply: (@pperm_trans (s4++s5)); first by apply: IH1 E1 E.
   by apply: IH2 E E2.
 - by move=>x [].
-- move=>x t1 t2 H IH y s1 s2 p1 p2 E1 E2.
-  case: s1 E1=>[|b s1] /=; case: p1 E2=>[|c p1] /= E1 E2.
-  - by case: E1 E2=><- <- [<-].
-  - apply: (@perm_trans (p1 ++ c :: p2))=>//.
-    by case: E1 H=><- ->; case: E2=><- ->.
-  - case: E1 E2 H=><- <- [<-] ->; apply: (@perm_trans (s1 ++ x:: s2)).
-    by apply: perm_cons_cat_consL.
-  case: E1 E2 H IH=><- -> [<-] -> H IH.
-  by apply: permutation_skip=>//; apply: IH.
-move=>x y p1 p2 H IH z s1 t1 s2 t2 E1 E2.
-case: s1 E1 H IH=>[|b s1]; case: s2 E2=>[|c s2]=>/=.
-- by case=><- <- [<-] <- H IH; apply: permutation_skip.
-- case=><-; case: s2=>[|b s2] /=.
-  - by case=><- <-; case=><- H IH; apply: permutation_skip H.
-  case=><- -> [<-] <- H IH.
-  by apply: permutation_skip=>//; apply: perm_trans H _.
-- case=><- <- [<-]; case: s1=>[|a s1] /=.
-  - by case=><- H IH; apply: permutation_skip.
-  by case=><- -> H IH; apply: permutation_skip=>//; apply: perm_trans H.
-case=><-; case: s2=>[|a s2] /=; case: s1=>[|d s1] /=.
-- by case=><- <- [<-] <- <- H IH; apply: permutation_skip.
-- case=><- <- [<-] <- -> H IH.
-  apply: (@perm_trans (x::y::s1 ++ t1)); first by apply: permutation_swap.
-  by apply: permutation_skip=>//; apply: perm_trans H.
-- case=><- -> [<-] <- <- H IH.
-  apply: (@perm_trans (y::x::s2++t2)); last by apply: permutation_swap.
-  by apply: permutation_skip=>//; apply: perm_trans H _.
-case=><- -> [<-] <- -> H IH.
-apply: (@perm_trans (x::y::s1++t1)); first by apply: permutation_swap.
-by apply: permutation_skip=>//; apply: permutation_skip=>//; apply: IH.
+- move=>x t1 t2 H IH y [|b s1] s2 [|c p1] p2 /= [E1 E2] [E3 E4]; subst x;
+    rewrite ?E1 ?E2 ?E3 ?E4 in H * =>//.
+  - by subst y; apply: pperm_trans H _.
+  - by apply: pperm_trans H.
+  by apply: permutation_skip=>//; apply: IH E2 E4.
+move=>x y p1 p2 H IH z [|b s1] t1 [|c s2] t2 /= [E1 E2] [E3 E4]; subst x y;
+  rewrite -?E2 -?E4 in H IH * =>//.
+- by apply: permutation_skip.
+- case: s2 E4=>/=[|a s2][<-]=>[|E4]; apply: permutation_skip=>//.
+  by subst p2; apply: pperm_trans H _; apply pperm_cons_catAC.
+- case: s1 E2=>/=[|a s1][<-]=>[|E2]; apply: permutation_skip=>//.
+  by subst p1; apply: pperm_trans H; apply pperm_cons_catCA.
+case: s1 E2=>/=[|a s1][->]=>E2; case: s2 E4=>/=[|d s2][->]=>E4;
+  rewrite ?E2 ?E4 in H IH *.
+- by apply: permutation_skip.
+- apply: (@pperm_trans [:: d, z & s2 ++ t2]); last by apply: permutation_swap.
+  by apply: permutation_skip=>//; apply/(pperm_trans H _ )/pperm_cons_catAC.
+- apply: (@pperm_trans [:: a, z & s1 ++ t1]); first by apply: permutation_swap.
+  by apply: permutation_skip=>//; apply/pperm_trans/H/pperm_cons_catCA.
+by apply: permutation_swap; apply: IH.
 Qed.
 
-Lemma perm_cons x s1 s2 : perm (x :: s1) (x :: s2) <-> perm s1 s2.
+Lemma pperm_cons x s1 s2 : perm (x :: s1) (x :: s2) <-> perm s1 s2.
 Proof.
-split; last by apply: permutation_skip.
-by move/(@perm_cat_consR [::] s1 [::] s2 x).
+by split; [apply/(@pperm_cat_consR [::] [::]) | apply: permutation_skip].
 Qed.
 
-Lemma perm_cons_cat_cons x s1 s2 s :
+Lemma pperm_cat2l s s1 s2: perm (s ++ s1) (s ++ s2) <-> perm s1 s2.
+Proof. by split; [elim: s=>// ??? /pperm_cons | apply: pperm_cat2lL]. Qed.
+
+Lemma pperm_cat2r s s1 s2 : perm (s1 ++ s) (s2 ++ s) <-> perm s1 s2.
+Proof.
+split; last by apply: pperm_cat2rL.
+by elim: s=>[|??? /pperm_cat_consR]; rewrite ?cats0.
+Qed.
+
+Lemma pperm_catAC s1 s2 s3 : perm ((s1 ++ s2) ++ s3) ((s1 ++ s3) ++ s2).
+Proof. by move=>*; rewrite -!catA pperm_cat2l. Qed.
+
+Lemma pperm_catCA s1 s2 s3 : perm (s1 ++ s2 ++ s3) (s2 ++ s1 ++ s3).
+Proof. by move=>*; rewrite !catA pperm_cat2r. Qed.
+
+Lemma pperm_cons_cat_cons x s1 s2 s :
         perm (x :: s) (s1 ++ x :: s2) <-> perm s (s1 ++ s2).
 Proof.
-split=>[|H]; first by by move/(@perm_cat_consR [::] s s1 s2 x).
-by apply: (@perm_trans (x :: s1++s2))=>//; apply: permutation_skip.
+by split; [apply: (@pperm_cat_consR [::]) | apply: pperm_cons_cat_consL].
 Qed.
 
-Lemma perm_cat_cons x s1 s2 t1 t2 :
+Lemma pperm_cat_cons x s1 s2 t1 t2 :
         perm (s1 ++ x :: t1) (s2 ++ x :: t2) <-> perm (s1 ++ t1) (s2 ++ t2).
 Proof.
-split=>[|H]; first by apply: perm_cat_consR.
-apply: (@perm_trans (x::s1++t1))=>//; apply: (@perm_trans (x::s2++t2))=>//.
-by apply/perm_cons.
+split=>[|H]; first by apply: pperm_cat_consR.
+apply: (@pperm_trans (x::s1++t1))=>//; apply: (@pperm_trans (x::s2++t2))=>//.
+by apply/pperm_cons.
 Qed.
-
-Lemma perm_cat2l s1 s2 s3: perm (s1 ++ s2) (s1 ++ s3) <-> perm s2 s3.
-Proof.
-split; last by apply: perm_cat2lL.
-elim: s1 s2 s3=>[|x s1 IH] s2 s3 //= H.
-by apply: IH; move/perm_cons: H.
-Qed.
-
-Lemma perm_cat2r s1 s2 s3 : perm (s2 ++ s1) (s3 ++ s1) <-> perm s2 s3.
-Proof.
-split; last by apply: perm_cat2rL.
-elim: s1 s2 s3=>[|x s1 IH] s2 s3 /=; first by rewrite !cats0.
-by move=>H; apply: IH; apply: perm_cat_consR H.
-Qed.
-
-Lemma perm_catAC s1 s2 s3 : perm ((s1 ++ s2) ++ s3) ((s1 ++ s3) ++ s2).
-Proof. by move=>*; rewrite -!catA perm_cat2l. Qed.
-
-Lemma perm_catCA s1 s2 s3 : perm (s1 ++ s2 ++ s3) (s2 ++ s1 ++ s3).
-Proof. by move=>*; rewrite !catA perm_cat2r. Qed.
 
 End Permutations.
 
-Hint Resolve perm_refl perm_catC perm_cons_catCA
-             perm_cons_catAC perm_catAC perm_catCA.
-
+Hint Resolve pperm_refl pperm_catC pperm_cons_catCA
+             pperm_cons_catAC pperm_catAC pperm_catCA : core.
 
 (* perm and map *)
-
-Lemma perm_map A B (f : A -> B) (s1 s2 : seq A) :
+Lemma pperm_map A B (f : A -> B) (s1 s2 : seq A) :
         perm s1 s2 -> perm (map f s1) (map f s2).
 Proof.
-set P := fun s1 s2 => perm (map f s1) (map f s2).
-suff {s1 s2} L: forall s1 s2, perm s1 s2 -> P s1 s2 by apply: L.
-apply: perm_ind2=>//; last 1 first.
-- move=>s2 s1 s3 _ IH1 _ IH2.
-  by apply: perm_trans IH1 IH2.
-- by move=>x s1 s2 H IH; rewrite /P perm_cons.
-move=>x1 x2 s1 s2 H IH.
-have L: perm [:: f x2, f x1 & map f s1] ([:: f x1] ++ [:: f x2 & map f s1]).
-- by apply/perm_cons_cat_cons.
-by apply: perm_trans L _; rewrite !perm_cons.
+elim=>[//|||??? _ IH1 _ IH2]*;
+by [apply/pperm_cons | apply/permutation_swap | apply/(pperm_trans IH1 IH2)].
 Qed.
 
 (* mapping to ssreflect decidable perm *)
-
 Lemma perm_eq_perm (A : eqType) (s1 s2 : seq A) :
         reflect (perm s1 s2) (perm_eq s1 s2).
 Proof.
 apply: (iffP idP); last first.
-- elim: s1 s2 /; last 1 first.
-  - by move=>s1 s2 t _ H2 _; apply: perm_eq_trans H2.
-  - by move=>s1 s2 ->->.
-  - by move=>s1 s2 x t1 t2 ->-> H1 H2; rewrite seq.perm_cons.
-  move=>s1 s2 x y t ->->.
-  by rewrite -(perm_rot 1) /rot /= seq.perm_cons seq.perm_catC.
-elim: s1 s2=>[|x s1 IH] /= s2.
-- move/perm_eq_mem=>H; apply/perm_nil.
-  by case: s2 H=>// a s2 /(_ a); rewrite inE eq_refl.
-move=>H; move: (perm_eq_mem H x); rewrite inE eq_refl; move/esym=>/= H'.
-move/(perm_eq_trans H): {H} (perm_to_rem H'); rewrite seq.perm_cons.
-move/IH/(perm_cons x)=>H; apply: perm_trans H _.
-elim: s2 x H'=>[|y s2 IH2] //= x.
-rewrite inE; case/orP; first by move/eqP=><-; rewrite eq_refl.
-case: eqP=>[->//|_ H]; move/(perm_cons y): (IH2 _ H).
-by apply: perm_trans; apply: permutation_swap.
+- elim=>[|||??? _ H1 _ H2]*.
+  - by apply seq.perm_refl.
+  - by rewrite seq.perm_cons.
+  - by rewrite -![[:: _, _ & _]]/([::_] ++ [::_] ++ _) seq.perm_catCA;
+       rewrite !seq.perm_cat2l.
+  by apply: seq.perm_trans H1 H2.
+elim: s2 s1 =>[s1 /seq.perm_size/size0nil->// | x s2 IH s1 H].
+move: (seq.perm_mem H x); rewrite mem_head=>H'; move: H' H.
+move/splitPr=>[p1 p2]; rewrite -cat1s seq.perm_catCA seq.perm_cons=>/IH.
+by rewrite -[_::s2]cat0s pperm_cat_cons.
 Qed.
-
