Core/stsep.v
@@ -3,26 +3,27 @@ From fcsl Require Import pred pcm unionmap heap.
 From HTT Require Import stmod.
 Set Implicit Arguments.
 Unset Strict Implicit.
-Unset Printing Implicit Defensive. 
+Unset Printing Implicit Defensive.
 
-Delimit Scope stsep_scope with stsep. 
+Declare Scope stsep_scope.
+Delimit Scope stsep_scope with stsep.
 Open Scope stsep_scope.
 
 Definition star (p1 p2 : Pred heap) : Pred heap :=
   [Pred h | exists h1, exists h2, h = h1 \+ h2 /\ h1 \In p1 /\ h2 \In p2].
-Definition emp : Pred heap := eq^~ Unit. 
+Definition emp : Pred heap := eq^~ Unit.
 Definition top : Pred heap := PredT.
 
-Notation "p1 '#' p2" := (star p1 p2) 
+Notation "p1 '#' p2" := (star p1 p2)
   (at level 57, right associativity) : rel_scope.
 
-Definition lolli (p : _ -> Prop) q (i m : heap) := 
-  forall i1 h, i = i1 \+ h -> valid i -> p i1 -> 
+Definition lolli (p : _ -> Prop) q (i m : heap) :=
+  forall i1 h, i = i1 \+ h -> valid i -> p i1 ->
     exists m1, m = m1 \+ h /\ valid m /\ q i1 m1.
 
 Notation "p '--o' q"   := (lolli p q) (at level 75) : stsep_scope.
 
-Lemma antiframe p q i m h : 
+Lemma antiframe p q i m h :
         valid (i \+ h) -> (p --o q) (i \+ h) (m \+ h) -> (p --o q) i m.
 Proof.
 move=>D1 H i2 m2 E D2 H1; rewrite {i}E in H D1 D2 *.
@@ -32,8 +33,8 @@ by rewrite E in D3; rewrite (validL D3).
 Qed.
 
 (* p --o q is local *)
-Lemma locality p q i1 m h : 
-        valid (i1 \+ h) -> (p # top) i1 -> (p --o q) (i1 \+ h) m -> 
+Lemma locality p q i1 m h :
+        valid (i1 \+ h) -> (p # top) i1 -> (p --o q) (i1 \+ h) m ->
           exists m1, m = m1 \+ h /\ valid m /\ (p --o q) i1 m1.
 Proof.
 move=>D [h1][h2][E][H1] _ H2; rewrite {i1}E in D H2 *.
@@ -49,22 +50,22 @@ Proof. by case=>i1 [i2][->][H] _; rewrite -joinA; exists i1, (i2 \+ j). Qed.
 (* Separation monad *)
 (********************)
 
-Definition fr A (s : spec A) : spec A := 
+Definition fr A (s : spec A) : spec A :=
   (s.1 # top, fun x => s.1 --o s.2 x).
 
 Prenex Implicits fr.
 
 Notation "[ s ]" := (fr s).
 
-Definition STbin A (s : spec A) := STspec [s]. 
+Definition STbin A (s : spec A) := STspec [s].
 
 (* hide the spec *)
 Inductive ST A := with_spec (s : spec A) of STbin s.
 
 Definition spec_of A (e : ST A) := let: with_spec s _ := e in s.
-Definition pre_of A := [fun e : ST A => (spec_of e).1]. 
-Definition post_of A := [fun e : ST A => (spec_of e).2]. 
-Definition code_of A (e : ST A) := 
+Definition pre_of A := [fun e : ST A => (spec_of e).1].
+Definition post_of A := [fun e : ST A => (spec_of e).2].
+Definition code_of A (e : ST A) :=
   let: with_spec _ c := e return STbin (spec_of e) in c.
 
 Arguments pre_of {A}.
@@ -76,8 +77,8 @@ Coercion with_spec : STbin >-> ST.
 
 Section SepReturn.
 Variable (A : Type) (x : A).
- 
-Definition ret_s : spec A := (emp, fun y i m => m = i /\ y = Val x). 
+
+Definition ret_s : spec A := (emp, fun y i m => m = i /\ y = Val x).
 
 Lemma retP : Model.conseq (Model.ret_s x) [ret_s].
 Proof.
@@ -90,12 +91,12 @@ Definition ret := with_spec _ (Model.Do (Model.ret x) retP).
 End SepReturn.
 
 
-Section SepBind. 
-Variables (A B : Type) (e1 : ST A) (e2 : A -> ST B). 
-Notation s1 := (spec_of e1). 
-Notation s2 := (fun x => spec_of (e2 x)). 
+Section SepBind.
+Variables (A B : Type) (e1 : ST A) (e2 : A -> ST B).
+Notation s1 := (spec_of e1).
+Notation s2 := (fun x => spec_of (e2 x)).
 
-Definition bind_s : spec B := 
+Definition bind_s : spec B :=
   (Model.bind_pre [s1] (fr \o s2), Model.bind_post [s1] (fr \o s2)).
 
 Lemma bindP : Model.conseq (Model.bind_s [s1] (fr \o s2)) [bind_s].
@@ -110,8 +111,8 @@ case: H=>[[x][h][]|[e][->]]; case/(locality D1 H1)=>h1 [->][D2] T2.
   by exists m1; do !split=>//; left; exists x; exists h1.
 by exists h1; do !split=>//; right; exists e.
 Qed.
-  
-Definition bind := 
+
+Definition bind :=
   with_spec _ (Model.Do (Model.bind (code_of e1) (fun x => code_of (e2 x))) bindP).
 
 End SepBind.
@@ -120,14 +121,14 @@ End SepBind.
 Definition verify'' A (s : spec A) i (r : ans A -> heap -> Prop) :=
   valid i -> s.1 i /\ forall y m, s.2 y i m -> valid m -> r y m.
 
-Definition verify' A (e : ST A) i r := verify'' [spec_of e] i r. 
+Definition verify' A (e : ST A) i r := verify'' [spec_of e] i r.
 
 Notation verify i e r := (@verify' _ e i r).
 
 Section SepFrame.
-Variables (A : Type) (e : ST A). 
+Variables (A : Type) (e : ST A).
 
-Lemma frame i j (r : ans A -> heap -> Prop) : 
+Lemma frame i j (r : ans A -> heap -> Prop) :
         verify i e (fun y m => valid (m \+ j) -> r y (m \+ j)) ->
         verify (i \+ j) e r.
 Proof.
@@ -140,28 +141,28 @@ Qed.
 Lemma frame0 i r : verify'' (spec_of e) i r -> verify i e r.
 Proof.
 move=>H D; case: (H D)=>H1 H2.
-split=>[|y m]; first by exists i, Unit; rewrite unitR. 
+split=>[|y m]; first by exists i, Unit; rewrite unitR.
 move/(_ i Unit); rewrite unitR; case/(_ (erefl _) D H1)=>m1.
 by rewrite unitR=>[[<-]][_]; apply: H2.
 Qed.
 
 Lemma frame1 i (r : ans A -> heap -> Prop) :
-        verify'' (spec_of e) Unit (fun y m => valid (m \+ i) -> r y (m \+ i)) -> 
+        verify'' (spec_of e) Unit (fun y m => valid (m \+ i) -> r y (m \+ i)) ->
         verify i e r.
 Proof. by move=>H; rewrite -[i]unitL; apply: frame; apply: frame0. Qed.
 
 End SepFrame.
 
-Definition conseq A (e : ST A) (s : spec A) := 
+Definition conseq A (e : ST A) (s : spec A) :=
   forall i, s.1 i -> verify i e (fun y m => s.2 y i m).
 
 (*
-Local Notation conseq1 e s := 
-  (conseq e (let 'pair x _ := s in x) 
+Local Notation conseq1 e s :=
+  (conseq e (let 'pair x _ := s in x)
             (let 'pair _ x := s in x)).
 *)
 
-Lemma conseq_refl A (e : ST A) : conseq e (spec_of e). 
+Lemma conseq_refl A (e : ST A) : conseq e (spec_of e).
 Proof. by case: e=>s e i H; apply: frame0. Qed.
 
 Hint Resolve conseq_refl : core.
@@ -173,7 +174,7 @@ Lemma doP : Model.conseq [spec_of e] [s2].
 Proof.
 move=>i H D; split=>[|y m {H D} /=].
 - case: H D=>i1 [i2][->][H] _ D.
-  by case: (@pf i1 H (validL D))=>H1 _; apply: fr_pre. 
+  by case: (@pf i1 H (validL D))=>H1 _; apply: fr_pre.
 move=>S D i1 i2 E D2 H2; rewrite {i}E in D S D2 H2.
 case: (@pf i1 H2 (validL D2))=>H1 T1.
 case: (locality D2 H1 S)=>m1 [->][D3] {S}.
@@ -187,16 +188,16 @@ End SepConseq.
 Notation "'Do' e" := (@do' _ _ e _) (at level 80).
 
 Section SepRead.
-Variables (A : Type) (x : ptr). 
+Variables (A : Type) (x : ptr).
 
-Definition read_s : spec A := 
+Definition read_s : spec A :=
   (fun i => exists v : A, i = x :-> v,
    fun y i m => i = m /\ forall v, i = x :-> v -> y = Val v).
 
 Lemma readP : Model.conseq (Model.read_s A x) [read_s].
 Proof.
 move=>i H D; split=>[|{H D} y _ [->] H _ i1 h E1 D E2].
-- case: H D=>i1 [i2][->][[v]] -> _ D /=. 
+- case: H D=>i1 [i2][->][[v]] -> _ D /=.
   rewrite domPtUn inE /= D eq_refl; split=>//.
   by exists v; rewrite findPtUn.
 move: E1 E2 H D=>-> [v ->] H D; exists (x :-> v); do 3!split=>//.
@@ -209,10 +210,10 @@ Definition read := with_spec _ (Model.Do (Model.read A x) readP).
 End SepRead.
 
 
-Section SepWrite. 
+Section SepWrite.
 Variables (A : Type) (x : ptr) (v : A).
- 
-Definition write_s : spec unit := 
+
+Definition write_s : spec unit :=
   (fun i => exists B : Type, exists y : B, i = x :-> y,
    fun y i m => y = Val tt /\ m = x :-> v).
 
@@ -238,13 +239,13 @@ Qed.
 
 Definition write := with_spec _ (Model.Do (Model.write x v) writeP).
 
-End SepWrite. 
+End SepWrite.
 
 
 Section SepAlloc.
 Variables (A : Type) (v : A).
-  
-Definition alloc_s : spec ptr :=  
+
+Definition alloc_s : spec ptr :=
   (emp, fun y i m => exists x, y = Val x /\ m = x :-> v).
 
 Lemma allocP : Model.conseq (Model.alloc_s v) [alloc_s].
@@ -265,10 +266,10 @@ Definition alloc := with_spec _ (Model.Do (Model.alloc v) allocP).
 End SepAlloc.
 
 
-Section SepBlockAlloc.  
-Variables (A : Type) (v : A) (n : nat). 
+Section SepBlockAlloc.
+Variables (A : Type) (v : A) (n : nat).
 
-Definition allocb_s : spec ptr := 
+Definition allocb_s : spec ptr :=
   (emp, fun y i m => exists x:ptr, y = Val x /\ m = updi x (nseq n v)).
 
 Lemma allocbP : Model.conseq (Model.allocb_s v n) [allocb_s].
@@ -288,7 +289,7 @@ End SepBlockAlloc.
 Section SepDealloc.
 Variable x : ptr.
 
-Definition dealloc_s : spec unit := 
+Definition dealloc_s : spec unit :=
   (fun i => exists A : Type, exists v:A, i = x :-> v,
    fun y i m => y = Val tt /\ m = Unit).
 
@@ -308,9 +309,9 @@ End SepDealloc.
 
 Section SepThrow.
 Variables (A : Type) (e : exn).
- 
-Definition throw_s : spec A := 
-  (emp, fun y i m => m = i /\ y = Exn e). 
+
+Definition throw_s : spec A :=
+  (emp, fun y i m => m = i /\ y = Exn e).
 
 Lemma throwP : Model.conseq (Model.throw_s A e) [throw_s].
 Proof.
@@ -324,12 +325,12 @@ End SepThrow.
 
 
 Section SepTry.
-Variables (A B : Type) (e : ST A) (e1 : A -> ST B) (e2 : exn -> ST B). 
+Variables (A B : Type) (e : ST A) (e1 : A -> ST B) (e2 : exn -> ST B).
 Notation s := (spec_of e).
 Notation s1 := (fun x => spec_of (e1 x)).
 Notation s2 := (fun x => spec_of (e2 x)).
 
-Definition try_s : spec B := 
+Definition try_s : spec B :=
   (Model.try_pre [s] (fr \o s1) (fr \o s2),
    Model.try_post [s] (fr \o s1) (fr \o s2)).
 
@@ -342,15 +343,15 @@ move=>i H D; split=>[|{H D} y m H1 D1 i1 h E1 D2 /= [H2][H3] H4].
   by apply: fr_pre.
 rewrite {i}E1 /= in H1 D2.
 case: H1=>[[x]|[x]][h1][];
-case/(locality D2 H2)=>m1 [->][D3] T1; move: (T1); 
-[move/H3 | move/H4]=>T'; case/(locality D3 T')=>m2 [->][D4] T2; 
-exists m2; do 2!split=>//; [left | right]; 
+case/(locality D2 H2)=>m1 [->][D3] T1; move: (T1);
+[move/H3 | move/H4]=>T'; case/(locality D3 T')=>m2 [->][D4] T2;
+exists m2; do 2!split=>//; [left | right];
 by exists x, m1.
 Qed.
 
-Definition ttry := 
-  with_spec _ (Model.Do (Model.try (code_of e) 
-                                   (fun x => code_of (e1 x)) 
+Definition ttry :=
+  with_spec _ (Model.Do (Model.try (code_of e)
+                                   (fun x => code_of (e1 x))
                                    (fun x => code_of (e2 x))) tryP).
 
 End SepTry.
@@ -367,23 +368,23 @@ End SepFix.
 (* Notation to move from binary posts to unary ones *)
 (****************************************************)
 
-Definition logvar {B A} (s : A -> spec B) : spec B := 
-  (fun i => exists x : A, let 'pair p _ := s x in p i, 
+Definition logvar {B A} (s : A -> spec B) : spec B :=
+  (fun i => exists x : A, let 'pair p _ := s x in p i,
    fun y i m => forall x : A, let 'pair _ q := s x in q y i m).
 
-Definition binarify {A} (p : pre) (q : ans A -> pre) : spec A := 
+Definition binarify {A} (p : pre) (q : ans A -> pre) : spec A :=
   (p, fun y i m => p i -> q y m).
 
-Notation "'STsep' ( p , q ) " := (STbin (binarify p q)) (at level 0).  
+Notation "'STsep' ( p , q ) " := (STbin (binarify p q)) (at level 0).
 
 Notation "{ x .. y }, 'STsep' ( p , q ) " :=
   (STbin (logvar (fun x => .. (logvar (fun y => binarify p q)) .. )))
    (at level 0, x binder, y binder, right associativity).
 
 
-Notation "x '<--' c1 ';' c2" := (bind c1 (fun x => c2)) 
+Notation "x '<--' c1 ';' c2" := (bind c1 (fun x => c2))
   (at level 78, right associativity) : stsep_scope.
-Notation "c1 ';;' c2" := (bind c1 (fun _ => c2)) 
+Notation "c1 ';;' c2" := (bind c1 (fun _ => c2))
   (at level 78, right associativity) : stsep_scope.
 Notation "'!' x" := (read _ x) (at level 50) : stsep_scope.
 Notation "e1 '::=' e2" := (write e1 e2) (at level 60) : stsep_scope.
